@prefix adms: <http://www.w3.org/ns/adms#> .
@prefix dc: <http://purl.org/dc/elements/1.1/> .
@prefix dcat: <http://www.w3.org/ns/dcat#> .
@prefix dct: <http://purl.org/dc/terms/> .
@prefix ecm4m-voc: <https://purl.org/ecm4m/vocs/> .
@prefix euvoc: <http://publications.europa.eu/ontology/euvoc#> .
@prefix foaf: <http://xmlns.com/foaf/0.1/> .
@prefix org: <http://www.w3.org/ns/org#> .
@prefix owl: <http://www.w3.org/2002/07/owl#> .
@prefix pav: <http://purl.org/pav/> .
@prefix prov: <http://www.w3.org/ns/prov#> .
@prefix qb: <http://purl.org/linked-data/cube#> .
@prefix rdf: <http://www.w3.org/1999/02/22-rdf-syntax-ns#> .
@prefix rdfs: <http://www.w3.org/2000/01/rdf-schema#> .
@prefix schema: <http://schema.org/> .
@prefix sh: <http://www.w3.org/ns/shacl#> .
@prefix skos: <http://www.w3.org/2004/02/skos/core#> .
@prefix skosthes: <http://purl.org/iso25964/skos-thes#> .
@prefix skosxl: <http://www.w3.org/2008/05/skos-xl#> .
@prefix xsd: <http://www.w3.org/2001/XMLSchema#> .

<https://purl.org/ecm4m/vocs> a skos:ConceptScheme;
  dct:created "2022-06-01T00:00:00+00:00"^^xsd:datetime;
  dct:creator <https://orcid.org/0000-0002-0972-6321>;
  dct:description "Collection of some EarthCube M4M vocabularies.";
  dct:hasVersion "0.1.0";
  dct:modified "2022-09-08T11:15:14-07:00"^^xsd:datetime;
  dct:rights <https://spdx.org/licenses/CC0-1.0>;
  dct:title "Example containing some M4M vocabularies";
  skos:hasTopConcept ecm4m-voc:Non-PolishedSectionContainerType, ecm4m-voc:Non-PolishedSectionSampleType,
    ecm4m-voc:PolishedSectionContainerType, ecm4m-voc:PolishedSectionSampleType;
  skos:prefLabel "Example containing some M4M vocabularies";
  foaf:homepage <https://github.com/go-fair-us/EarthCubeM4M> .

ecm4m-voc:Non-PolishedSectionSampleType a skos:Concept;
  skos:definition "Set of terms describing the sample types for non-polished sections"@en;
  skos:inScheme <https://purl.org/ecm4m/vocs>;
  skos:narrower ecm4m-voc:aggregate, ecm4m-voc:atomprobetip, ecm4m-voc:chip, ecm4m-voc:fibsection,
    ecm4m-voc:liquid, ecm4m-voc:microtomeslices, ecm4m-voc:particle, ecm4m-voc:powder,
    ecm4m-voc:residue;
  skos:prefLabel "Non-Polished Section Sample Type"@en;
  skos:topConceptOf <https://purl.org/ecm4m/vocs> .

ecm4m-voc:powder a skos:Concept;
  skos:broader ecm4m-voc:Non-PolishedSectionSampleType;
  skos:definition "Powders are samples that have been intentionally modified to reduce the average particle size. Powders can be generated by pulverizing particles, chips, and/or aggregate samples."@en;
  skos:inScheme <https://purl.org/ecm4m/vocs>;
  skos:prefLabel "powder"@en .

ecm4m-voc:aggregate a skos:Concept;
  skos:broader ecm4m-voc:Non-PolishedSectionSampleType;
  skos:definition "Aggregate samples are collections of particles; the particles in aggregate samples have not been intentionally modified. The particles in aggregate samples do not necessarily have any relationship to each other aside from being returned OSIRIS-REx material."@en;
  skos:inScheme <https://purl.org/ecm4m/vocs>;
  skos:prefLabel "aggregate"@en .

ecm4m-voc:chip a skos:Concept;
  skos:broader ecm4m-voc:Non-PolishedSectionSampleType;
  skos:definition "A chip is a piece intentionally broken off a particle or a piece that is observed and documented to have broken off a particle."@en;
  skos:inScheme <https://purl.org/ecm4m/vocs>;
  skos:prefLabel "chip"@en .

ecm4m-voc:particle a skos:Concept;
  skos:broader ecm4m-voc:Non-PolishedSectionSampleType;
  skos:definition "A particle is a competent individual geologic sample of any size."@en;
  skos:inScheme <https://purl.org/ecm4m/vocs>;
  skos:prefLabel "particle"@en .

ecm4m-voc:liquid a skos:Concept;
  skos:broader ecm4m-voc:Non-PolishedSectionSampleType;
  skos:definition "Solution that a solid sample has been extracted into."@en;
  skos:inScheme <https://purl.org/ecm4m/vocs>;
  skos:prefLabel "liquid"@en .

ecm4m-voc:fibsection a skos:Concept;
  skos:broader ecm4m-voc:Non-PolishedSectionSampleType;
  skos:definition "FIB sections are milled out of samples with a focused ion beam (FIB)."@en;
  skos:inScheme <https://purl.org/ecm4m/vocs>;
  skos:prefLabel "fibsection"@en .

ecm4m-voc:atomprobetip a skos:Concept;
  skos:broader ecm4m-voc:Non-PolishedSectionSampleType;
  skos:definition "Atom probe tips are needle-shaped samples milled out of samples with a focused ion beam (FIB)."@en;
  skos:inScheme <https://purl.org/ecm4m/vocs>;
  skos:prefLabel "atomprobetip"@en .

ecm4m-voc:microtomeslices a skos:Concept;
  skos:broader ecm4m-voc:Non-PolishedSectionSampleType;
  skos:definition "Microtome slices are prepared by cutting a particle embedded in an epoxy bullet into numerous slices with a ultramicrotome. Multiple slices will be deposited onto a single TEM grid. When this happens the grid will be given a single sample name, not the individual slices within it."@en;
  skos:inScheme <https://purl.org/ecm4m/vocs>;
  skos:prefLabel "microtomeslices"@en .

ecm4m-voc:residue a skos:Concept;
  skos:broader ecm4m-voc:Non-PolishedSectionSampleType;
  skos:definition "Residues are solids leftover after dissolution of samples and subsequent chemical processing."@en;
  skos:inScheme <https://purl.org/ecm4m/vocs>;
  skos:prefLabel "residue"@en .

ecm4m-voc:Non-PolishedSectionContainerType a skos:Concept;
  skos:definition "Set of words describing the sample types for non-polished sections"@en;
  skos:inScheme <https://purl.org/ecm4m/vocs>;
  skos:narrower ecm4m-voc:aluminumcontainer, ecm4m-voc:aluminumwrapping, ecm4m-voc:customcontainer,
    ecm4m-voc:glassvial, ecm4m-voc:polycarbonatecontainer, ecm4m-voc:teflonbag;
  skos:prefLabel "Non-Polished Section Container Type"@en;
  skos:topConceptOf <https://purl.org/ecm4m/vocs> .

ecm4m-voc:aluminumcontainer a skos:Concept;
  skos:broader ecm4m-voc:Non-PolishedSectionContainerType;
  skos:inScheme <https://purl.org/ecm4m/vocs>;
  skos:prefLabel "aluminumcontainer"@en .

ecm4m-voc:glassvial a skos:Concept;
  skos:broader ecm4m-voc:Non-PolishedSectionContainerType;
  skos:inScheme <https://purl.org/ecm4m/vocs>;
  skos:prefLabel "glassvial"@en .

ecm4m-voc:teflonbag a skos:Concept;
  skos:broader ecm4m-voc:Non-PolishedSectionContainerType;
  skos:inScheme <https://purl.org/ecm4m/vocs>;
  skos:prefLabel "teflonbag"@en .

ecm4m-voc:polycarbonatecontainer a skos:Concept;
  skos:broader ecm4m-voc:Non-PolishedSectionContainerType;
  skos:inScheme <https://purl.org/ecm4m/vocs>;
  skos:prefLabel "polycarbonatecontainer"@en .

ecm4m-voc:aluminumwrapping a skos:Concept;
  skos:broader ecm4m-voc:Non-PolishedSectionContainerType;
  skos:inScheme <https://purl.org/ecm4m/vocs>;
  skos:prefLabel "aluminumwrapping"@en .

ecm4m-voc:customcontainer a skos:Concept;
  skos:broader ecm4m-voc:Non-PolishedSectionContainerType;
  skos:inScheme <https://purl.org/ecm4m/vocs>;
  skos:prefLabel "customcontainer"@en .

ecm4m-voc:PolishedSectionSampleType a skos:Concept;
  skos:definition "Set of words describing the sample types for polished sections"@en;
  skos:inScheme <https://purl.org/ecm4m/vocs>;
  skos:prefLabel "Polished Section Sample Type"@en;
  skos:topConceptOf <https://purl.org/ecm4m/vocs> .

ecm4m-voc:thinSection a skos:Concept;
  skos:broader ecm4m-voc:PolishedSectionSampletype;
  skos:definition "Samples mounted onto a glass slide and polished to a thickness of ~30 µm. Thin sections made at JSC are polished on both sides (the side adhered to the glass with epoxy and the exposed side)."@en;
  skos:inScheme <https://purl.org/ecm4m/vocs>;
  skos:prefLabel "thinSection"@en .

ecm4m-voc:thickSection a skos:Concept;
  skos:broader ecm4m-voc:PolishedSectionSampletype;
  skos:definition "Samples may be polished on only one side. The sample thickness is greater than a standard thin section (~30 µm) – the desired thickness should be specified. Thick sections are typically mounted onto a glass slide when prepared at JSC thick sections on a glass slide are polished on both sides."@en;
  skos:inScheme <https://purl.org/ecm4m/vocs>;
  skos:prefLabel "thickSection"@en .

ecm4m-voc:pottedButt a skos:Concept;
  skos:broader ecm4m-voc:PolishedSectionSampletype;
  skos:definition "Potted butts are sample pieces mounted in epoxy from which multiple thin or thick sections can be made. In the event that it is not possible to make a thin or thick section of any particle, potted butts may be the primary sample preparation and holder for in situ analyses."@en;
  skos:inScheme <https://purl.org/ecm4m/vocs>;
  skos:prefLabel "pottedButt"@en .

ecm4m-voc:pressedGrainsEpoxy a skos:Concept;
  skos:broader ecm4m-voc:PolishedSectionSampletype;
  skos:definition "Grain mounts typically include multiple pieces of sample mounted (in epoxy or metal) and polished on one exposed side."@en;
  skos:inScheme <https://purl.org/ecm4m/vocs>;
  skos:prefLabel "pressedGrainsEpoxy"@en .

ecm4m-voc:pressedGrainsMetal a skos:Concept;
  skos:broader ecm4m-voc:PolishedSectionSampletype;
  skos:definition "Grain mounts typically include multiple pieces of sample mounted (in epoxy or metal) and polished on one exposed side."@en;
  skos:inScheme <https://purl.org/ecm4m/vocs>;
  skos:prefLabel "pressedGrainsMetal"@en .

ecm4m-voc:PolishedSectionContainerType a skos:Concept;
  skos:definition "Set of words describing the sample types for polished sections"@en;
  skos:inScheme <https://purl.org/ecm4m/vocs>;
  skos:narrower ecm4m-voc:ps_aluminumcontainer, ecm4m-voc:ps_aluminumwrapping, ecm4m-voc:ps_customcontainer,
    ecm4m-voc:ps_polycarbonatecontainer, ecm4m-voc:ps_teflonbag;
  skos:prefLabel "Polished Section Container Type"@en;
  skos:topConceptOf <https://purl.org/ecm4m/vocs> .

ecm4m-voc:ps_aluminumcontainer a skos:Concept;
  skos:broader ecm4m-voc:PolishedSectionContainerType;
  skos:inScheme <https://purl.org/ecm4m/vocs>;
  skos:prefLabel "aluminumcontainer"@en .

ecm4m-voc:ps_teflonbag a skos:Concept;
  skos:broader ecm4m-voc:PolishedSectionContainerType;
  skos:inScheme <https://purl.org/ecm4m/vocs>;
  skos:prefLabel "teflonbag"@en .

ecm4m-voc:ps_polycarbonatecontainer a skos:Concept;
  skos:broader ecm4m-voc:PolishedSectionContainerType;
  skos:inScheme <https://purl.org/ecm4m/vocs>;
  skos:prefLabel "polycarbonatecontainer"@en .

ecm4m-voc:ps_aluminumwrapping a skos:Concept;
  skos:broader ecm4m-voc:PolishedSectionContainerType;
  skos:inScheme <https://purl.org/ecm4m/vocs>;
  skos:prefLabel "aluminumwrapping"@en .

ecm4m-voc:ps_customcontainer a skos:Concept;
  skos:broader ecm4m-voc:PolishedSectionContainerType;
  skos:inScheme <https://purl.org/ecm4m/vocs>;
  skos:prefLabel "customcontainer"@en .

ecm4m-voc:PolishedSectionSampletype skos:narrower ecm4m-voc:pottedButt, ecm4m-voc:pressedGrainsEpoxy,
    ecm4m-voc:pressedGrainsMetal, ecm4m-voc:thickSection, ecm4m-voc:thinSection .